Denotation/theories/ContextTypeDenotationTactics.v
@@ -9,6 +9,7 @@ From ContextLogic Require Import FormulaSyntax.
 (** ** Denotation formula normalization tactics *)
 
 Ltac normalize_denotation_formula_fv :=
+  unfold denot_guard_formula;
   repeat first
     [ rewrite formula_fv_true | rewrite formula_fv_false
     | rewrite formula_fv_and | rewrite formula_fv_or
@@ -34,6 +35,7 @@ Ltac normalize_denotation_formula_fv :=
     ?context_ty_lvars_fv.
 
 Ltac normalize_denotation_formula_fv_in H :=
+  unfold denot_guard_formula in H;
   repeat first
     [ rewrite formula_fv_true in H | rewrite formula_fv_false in H
     | rewrite formula_fv_and in H | rewrite formula_fv_or in H
